<script>
  function winhisback() {window.history.back();}
</script>
<style>
  body {font-family: Palatino}
  .goback {color: purple}
</style>
<title>Solutions of Selected Problems from Boyce/DiPrima "Elem. DEs & BVPs 5th Ed. Chapter 6 Sec. 2"</title>
$\require{cancel}$

## <center>Selected Problem Solutions
<center>from</center>
### <center>Boyce, W. E. & R. C. DiPrima, 1992. <i>Elementary Differential Equations and</i><br><i>Boundary Value Problems, Fifth Edition</i>. John Wiley & Sons, New York.
### <center>Chapter 6, Section 2: The Laplace Transform, Solution of Initial Value Problems
### <center>&copy; 2019, 2025 by
### <center>[David Lawrence Goldsmith](https://www.linkedin.com/in/olydlg)
<center>for</center>
## <center>[SelectedSolutionsDotNet](https://olydlg.github.io/selectedsolutionsdotnet/)

<i>Notes: These solutions are provided "as-is," for informational purposes only, with no warranty of any kind, expressed or implied, including that of correctness, adequacy, and/or suitability for any purpose, whatsoever.</i> Corrections are welcome and should be emailed to selectedsolutionsdotnet@gmail.com.

Unless otherwise indicated, all inverse transforms are found using text Table 6.2.1, with the table entry number(s) (TE#) indicating the specific transform(s) used.

Purple font indicates clicking on the text will return you to your prior place.

### Contents
<table>
  <tr  style="border: none;">
    <td style="border: none;"><a href="#P2">Problem 2</a></td>
    <td style="border: none;"><a href="#P5">Problem 5</a></td>
    <td style="border: none;"><a href="#P8">Problem 8</a></td>
    <td style="border: none;"><a href="#P11">Problem 11</a></td>
    <td style="border: none;"><a href="#P14">Problem 14</a></td>
  </tr>
  <tr  style="border: none; background-color: white;">
    <td style="border: none;"><a href="#P17">Problem 17</a></td>
    <td style="border: none;"><a href="#P20">Problem 20</a></td>
    <td style="border: none;"><a href="#P23">Problem 23</a></td>
    <td style="border: none;"><a href="#P26">Problem 26</a></td>
    <td style="border: none;"><a href="#P27">Problem 27</a></td>
  </tr>
  <tr  style="border: none;">
    <td style="border: none;"><a href="#P30">Problem 30</a></td>
    <td style="border: none;"><a href="#P33">Problem 33</a></td>
    <td style="border: none;"><a href="#P36">Problem 36</a></td>
  </tr>
</table>

### Problems 2, 5, & 8: Find the inverse Laplace transform, $\mathcal{L}^{-1},$ of the given function

<a name="P2" class="goback" onclick="winhisback()">__2__)</a>
$\displaystyle \mathcal{F}(s) = \frac{4}{(s-1)^3}$

<b>Sln</b>: $\mathcal{L}^{-1}\left[\displaystyle \frac{4}{(s-1)^3}\right] = 2\mathcal{L}^{-1}\left[\displaystyle \frac{n!}{(s-a)^{n+1}}\right]$ where $n=2, a=1, \underset{\text{TE 11}}{=} \boxed{2t^2e^t}$
<br><br>

<a name="P5" class="goback" onclick="winhisback()">__5__)</a> 
$\displaystyle \mathcal{F}(s) = \frac{2s+2}{s^2 + 2s + 5}$

<b>Sln</b>: $\mathcal{L}^{-1}\left[\displaystyle \frac{2s+2}{s^2 + 2s + 5}\right] = 2\mathcal{L}^{-1}\left[\displaystyle \frac{s-(-1)}{(s-(-1))^2 + 2^2}\right] = 2\mathcal{L}^{-1}\left[\displaystyle \frac{s-a}{(s-a)^2 + b^2}\right]$ where $a=-1, b=2, \underset{\text{TE 10}}{=} \boxed{2e^{-t}\cos(2t)}$
<br><br>

<a name="P8" class="goback" onclick="winhisback()">__8__)</a>
$\displaystyle \mathcal{F}(s) = \frac{8s^2 - 4s + 12}{s(s^2+4)}$

$\begin{eqnarray} 
\textbf{Sln}\text{: }\mathcal{L}^{-1}\left[\displaystyle \frac{8s^2 - 4s + 12}{s(s^2+4)}\right] & = & \mathcal{L}^{-1}\left[\displaystyle \frac{A}s + \frac{Bs+C}{s^2+4}\right], \text{where } A+B = 8, C = -4, 4A = 12 \implies A = 3, B = 5, \\
& = & 3\mathcal{L}^{-1}\left[\displaystyle \frac1{s}\right] + 5\mathcal{L}^{-1}\left[\frac{s}{s^2+2^2}\right] - 2\mathcal{L}^{-1}\left[\frac{2}{s^2+2^2} \right] \\
& \underset{\text{TE 1, 6, 5}}{=} & \boxed{3 + 5\cos(2t) - 2\sin(2t)}
\end{eqnarray}$
<br><br>

### Problems 11, 14, 17, 20, & 23: Solve the given IVP, using the method of Laplace transforms

<a name="P11" class="goback" onclick="winhisback()">__11__)</a>
$y’’ - y’ -6y = 0,~~y(0) = 1,~~y’(0) = -1$

$\begin{eqnarray} 
\textbf{Sln}\text{: }\mathcal{L}[0] = 0 & = & \mathcal{L}\left[y’’ - y’ -6y\right] \\
& = & \left[s^2\mathcal{L}[y] - sy(0) - y’(0)\right] - \left[s\mathcal{L}[y] - y(0)\right] - 6\mathcal{L}[y] \\
& = & (s^2 - s - 6)\mathcal{L}[y] - s - (-1) + 1 \\
& = & (s^2 - s - 6)\mathcal{L}[y] - s + 2
\end{eqnarray}$

$\begin{eqnarray} \implies \mathcal{L}[y] = \displaystyle \frac{s-2}{s^2 - s - 6} \implies y = \mathcal{L}^{-1}\left[\displaystyle \frac{s-2}{s^2 - s - 6}\right] & = & \frac15\mathcal{L}^{-1}\left[\frac{1}{s-3}\right] + \frac45\mathcal{L}^{-1}\left[\frac{1}{s+2}\right] \\
& \underset{\text{TE 2}}{=} & \boxed{\frac{e^{3t} + 4e^{-2t}}{5}}
\end{eqnarray}$

$\checkmark: y(0) = \frac{1+4}{5} = 1~\checkmark \\
y’ = \displaystyle \frac{3e^{3t} - 8e^{-2t}}{5} \implies y’(0) = \frac{3-8}{5} = -1~\checkmark \\
y’’ = \displaystyle \frac{9e^{3t} + 16e^{-2t}}{5} \implies y’’ - y’ - 6y = \frac{(9-3-6)e^{3t} + (16 - (-8) - 24)e^{-2t}}{5} = 0~\checkmark$
<br><br>

<a name="P14" class="goback" onclick="winhisback()">__14__)</a>
$y’’ - 4y’ + 4y = 0,~~y(0) = 1,~~y’(0) = 1$

$\begin{eqnarray} 
\textbf{Sln}\text{: }\mathcal{L}[0] = 0 & = & \mathcal{L}\left[y’’ - 4y’ + 4y\right] \\
& = & [s^2\mathcal{L}[y] - s -1] - 4[s\mathcal{L}[y] - 1] + 4\mathcal{L}[y] \\
& = & (s^2 - 4s + 4)\mathcal{L}[y] - s + 3
\end{eqnarray}$

$\begin{eqnarray} \implies \mathcal{L}[y] = \displaystyle \frac{s-3}{(s-2)^2} \implies y & = & \mathcal{L}^{-1}\left[\displaystyle \frac{1}{s-2}\right] - \mathcal{L}^{-1}\left[\frac1{(s-2)^2}\right] \\
& \underset{\text{TE 2 & 11}}= & e^{2t} - te^{2t} = \boxed{(1-t)e^{2t}} 
\end{eqnarray}$

$\checkmark : y(0) = (1-0)e^{2(0)} = 1~\checkmark \\
y’ = 2(1-t)e^{2t} - e^{2t} = (1-2t)e^{2t} \implies y’(0) = (1-0)e^0 = 1~\checkmark \\
y’’ = 2(1-2t)e^{2t} - 2e^{2t} = -4te^{2t} \implies y’’ - 4y’ + 4y = -4te^{2t} - 4(1-2t)e^{2t} + 4(1-t)e^{2t} = (-4t + 8t - 4t - 4 + 4)e^{2t} = 0~\checkmark
$<br><br>

<a name="P17" class="goback" onclick="winhisback()">__17__)</a>
$y^{\text{iv}} - 4y’’’ + 6y’’ - 4y’ + y = 0,~~y(0) = 0,~~y’(0) = 1,~~y’’(0) = 0,~~y’’’(0) = 1$

$\begin{eqnarray} 
\textbf{Sln}\text{: }\mathcal{L}[0] = 0 & = & \mathcal{L}\left[y^{\text{iv}} - 4y’’’ + 6y’’ - 4y’ + y\right] \\
& = & [s^4\mathcal{L}[y] - s^3y(0) - s^2y’(0) - sy’’(0) - y’’’(0)] \\
& & - 4[s^3\mathcal{L}[y] - s^2y(0) - sy’(0) - y’’(0)] + 6[s^2\mathcal{L}[y] - sy(0) - y’(0)] - 4[s\mathcal{L}[y] - y(0)] + \mathcal{L}[y] \\
& = & (s^4 - 4s^3 + 6s^2 - 4s + 1)\mathcal{L}[y] - s^2 + 4s - 7 \\
\end{eqnarray}$

$\begin{eqnarray} \implies \mathcal{L}[y] = \displaystyle \frac{s^2 - 4s + 7}{(s-1)^4} \implies y & = & \mathcal{L}^{-1}\left[\displaystyle \frac{0}{s-1}\right] + \mathcal{L}^{-1}\left[\frac{1}{(s-1)^2}\right] + \mathcal{L}^{-1}\left[\frac{-2}{(s-1)^3}\right] + \mathcal{L}^{-1}\left[\frac{4}{(s-1)^4}\right] \\
& = & 0 + \mathcal{L}^{-1}\left[\frac{1!}{(s-1)^{1+1}}\right] - \mathcal{L}^{-1}\left[\frac{2!}{(s-1)^{2+1}}\right] + \frac23 \mathcal{L}^{-1}\left[\frac{3!}{(s-1)^{3+1}}\right] \\
& \underset{\text{TE 11}}{=} & te^t - t^2e^t +\frac23 t^3e^t = \boxed{\left(\frac23 t^3 - t^2 + t\right)e^t}
\end{eqnarray}$

$\checkmark$-step: Left for the reader
<br><br>

<a name="P20" class="goback" onclick="winhisback()">__20__)</a>
$y’’ + \omega^2y = \cos(2t),~~\omega^2 \ne 4,~~y(0) = 1,~~y’(0) = 0$

$\begin{eqnarray} 
\textbf{Sln}\text{: }\mathcal{L}[\cos(2t)] \underset{\text{TE 6}}{=} \frac{s}{s^2 + 4} & = & \mathcal{L}\left[y’’ + \omega^2y\right] \\
& = & [s^2\mathcal{L}[y] - sy(0) - y’(0)] + \omega^2\mathcal{L}[y] \\
& = & (s^2 + \omega^2)\mathcal{L}[y] - s \\
\end{eqnarray}$

$\implies \mathcal{L}[y] = \displaystyle \frac{s^3 + 5s}{(s^2+4)(s^2+\omega^2)} \underset{\because~\omega^2 \ne 4}{=} \left(\frac1{\omega^2-4}\right)\frac{s}{s^2+4} + \left(\frac{\omega^2-5}{\omega^2-4}\right)\frac{s}{s^2+\omega^2}$

$\begin{eqnarray}
\implies y & = & \displaystyle \left(\frac1{\omega^2-4}\right)\mathcal{L}^{-1}\left[\frac{s}{s^2+4}\right] + \left(\frac{\omega^2-5}{\omega^2-4}\right)\mathcal{L}^{-1}\left[\frac{s}{s^2+\omega^2}\right] \\
& \underset{\text{TE 6}}{=} & \displaystyle \boxed{\left(\frac1{\omega^2-4}\right)\cos(2t) + \left(\frac{\omega^2-5}{\omega^2-4}\right)\cos(\omega t)} \\
\end{eqnarray}$

$\checkmark: y(0) = \displaystyle \left(\frac1{\omega^2-4}\right) + \left(\frac{\omega^2-5}{\omega^2-4}\right) = \frac{\omega^2-4}{\omega^2-4} = 1~~\checkmark \\
y’(0) = -2 \displaystyle \left(\frac1{\omega^2-4}\right)\sin(2(0)) - \omega\left(\frac{\omega^2-5}{\omega^2-4}\right)\sin(\omega(0)) = 0 + 0 = 0 ~~\checkmark \\
\begin{eqnarray}
y’’+ \omega^2 y & = & -4\displaystyle \left(\frac1{\omega^2-4}\right)\cos(2t) - \cancel{\omega^2\left(\frac{\omega^2-5}{\omega^2-4}\right)\cos(\omega t)} + \omega^2 \displaystyle \left(\frac1{\omega^2-4}\right)\cos(2t) + \cancel{\omega^2\left(\frac{\omega^2-5}{\omega^2-4}\right)\cos(\omega t)} \\
& = & (\omega^2-4)\displaystyle \left(\frac1{\omega^2-4}\right)\cos(2t) \\
& = & \cos(2t)~~\checkmark
\end{eqnarray}$
<br><br>

<a name="P23" class="goback" onclick="winhisback()">__23__)</a>
$y’’ + 2y’ + y = 4e^{-t},~~y(0) = 2,~~y’(0) = -1$

$\begin{eqnarray} 
\textbf{Sln}\text{: }\mathcal{L}[4e^{-t}] \underset{\text{TE 2}}{=} \frac{4}{s + 1} & = & \mathcal{L}\left[y’’ + 2y’ + y\right] \\
& = & [s^2\mathcal{L}[y] - 2s + 1] + 2[s\mathcal{L}[y] - 2] + \mathcal{L}[y] \\
& = & (s^2 + 2s + 1)\mathcal{L}[y] - 2s - 3 \\
\end{eqnarray}$

$\implies \mathcal{L}[y] = \displaystyle \frac4{(s+1)^3} + \frac{2s+3}{(s+1)^2} = \frac{2s^2 + 5s + 7}{(s+1)^3} = \frac2{s+1} + \frac1{(s+1)^2} + \frac4{(s+1)^3}
$

$\begin{eqnarray}
\implies y(t) & = & \displaystyle 2\mathcal{L}^{-1}\left[\frac1{s-(-1)}\right] + \mathcal{L}^{-1}\left[\frac{1!}{(s-(-1))^{1+1}}\right] + 2\mathcal{L}^{-1}\left[\frac{2!}{(s-(-1))^{2+1}}\right] \\
& \underset{\text{TE 2 & 11}}{=} & 2e^{-t} + te^{-t} + 2t^2e^{-t} \\
& = & \boxed{(2 + t + 2t^2)e^{-t}}
\end{eqnarray}$

$\checkmark: y(0) = (2 + 0 + 2(0)^2)e^{-0} = 2~~\checkmark \\
y’(t) = (1+4t)e^{-t} - (2 + t + 2t^2)e^{-t} = (-1 + 3t - 2t^2)e^{-t} \implies y’(0) = -1~~\checkmark \\
y’’ = (3-4t)e^{-t} - (-1 + 3t - 2t^2)e^{-t} = (4 - 7t + 2t^2)e^{-t} \implies \\
y’’ + 2y’ + y = [4 - 7t + 2t^2 + 2(-1 + 3t - 2t^2) + 2 + t + 2t^2]e^{-t} = [(6-2) + (7-7)t + (4-4)t^2]e^{-t} = 4e^{-t}~~\checkmark$
<br><br>

<a name="P26" class="goback" onclick="winhisback()">__26__)</a>
For the IVP $y’’ + 4y = f(t) = \Bigg\{\!
\begin{array}{c c} 
t, & 0 \le t \lt 1, \\ 
1, & 1 \le t \lt \infty; 
\end{array} 
\!~~y(0) = 0,~~y’(0) = 0$, calculate $\mathcal{L}[y].$

<b>Sln:</b> The Laplace transform of the left hand side, with the specified initial conditions, is simply $s^2\mathcal{L}[y] + 4\mathcal{L}[y] = (s^2+4)\mathcal{L}[y];$the Laplace transform of the right hand side must be calculated from the definition:

$\begin{eqnarray}
\mathcal{L}[f(t)] & = & \displaystyle \int_0^1 te^{-st}dt + \int_1^{\infty}e^{-st}dt \\
& = & \left[\left(-\frac{t}{s}-\frac1{s^2}\right)e^{-st}\right]_0^1 + \left[-\frac1s e^{-st}\right]_1^{\infty} \\
& = & \left[\left(\cancel{-\frac1s} - \frac1{s^2}\right)e^{-s} + \frac1{s^2}\right] - \cancel{\frac1se^{-s\infty}} + \cancel{\frac1s e^{-s}} \\
& = & \frac{1-e^{-s}}{s^2}
\end{eqnarray}$

We thus have $(s^2+4)\mathcal{L}[y] = \displaystyle \frac{1-e^{-s}}{s^2} \implies \boxed{\mathcal{L}[y] = \frac{1-e^{-s}}{s^2(s^2+4)}}$
<br><br>

<a name="P27" class="goback" onclick="winhisback()">__27__)</a>
Calculate the Laplace transforms of the indicated functions from their Taylor series [about zero].

<b>a)</b> $\sin t$

<b>Sln</b>: The T. S. [about 0] of $\sin t = \displaystyle \sum_{n=0}^{\infty} \frac{(-1)^n t^{2n+1}}{(2n+1)!} \implies$<br>$\mathcal{L}[\sin t] = \displaystyle \sum_{n=0}^{\infty} \frac{(-1)^n}{(2n+1)!}\mathcal{L}[t^{2n+1}] = \sum_{n=0}^{\infty} \frac{(-1)^n}{\cancel{(2n+1)!}}\frac{\cancel{(2n+1)!}}{s^{2n+2}} = \frac1{s^2}\sum_{n=0}^{\infty} \left(-\frac1{s^2}\right)^n = \frac1{s^2}\frac1{1-(-1/s^2)}$ (because the sum is that of a geometric series of constant term 1 and common ratio $-1/s^2$, the sum of which is well-known to be $[1-(-1/s^2)]^{-1}$) $= \boxed{\frac1{s^2 + 1}}$ 
<br>

<b>c*)</b> $J_0(t) = \displaystyle \sum_{n=0}^{\infty} \frac{(-1)^n t^{2n}}{2^{2n}(n!)^2}$ and $J_0(\sqrt{t}) = \displaystyle \sum_{n=0}^{\infty} \frac{(-1)^n (\sqrt{t})^{2n}}{2^{2n}(n!)^2}$
<br>

<b>Sln</b>: The first part of this sub-problem is the most difficult&mdash;it is the main reason why this problem is "asterisked"&mdash;so we will save it for last. For $J_0(\sqrt{t})$ we have:

$\displaystyle \mathcal{L}[J_0(\sqrt t)]  =  \sum_{n=0}^{\infty}\frac{(-1)^n}{2^{2n}(n!)^2} \mathcal{L}[t^n]  \underset{\text{TE 3}}{=} \sum_{n=0}^{\infty}\frac{(-1)^n}{2^{2n}(n!)^2} \frac{n!}{s^{n+1}} = \frac1s \sum_{n=0}^{\infty}\frac{(-1)^n}{2^{2n}n!s^n}  = \frac1s \sum_{n=0}^{\infty}\frac{[1/(-4s)]^n}{n!} = \boxed{\frac{e^{-1/(4s)}}{s}}$

For $\mathcal{L}[J_0(t)]$, we will need the [general binomial series formula](https://en.wikipedia.org/wiki/Binomial_series):

$$(1+x)^{\alpha} = \sum_{n=0}^{\infty} \binom{\alpha}{n} x^n$$

valid for real $\alpha$, where $\displaystyle \binom{\alpha}{n} := \frac{\alpha(\alpha-1)(\alpha-2)\cdot\cdot\cdot(\alpha - n + 1)}{n!}$, and in particular the special case found [here](https://en.wikipedia.org/wiki/Binomial_theorem#Newton%27s_generalized_binomial_theorem):

$$(1-x)^{-1/2} = \sum_{n=0}^{\infty}\binom{n - \frac12}{n} x^n = \sum_{n=0}^{\infty}\frac{(n-\frac12)(n-\frac32)\cdot\cdot\cdot(\frac12)}{n!} x^n$$

With that in our toolkit, we proceed as before:

$\displaystyle \mathcal{L}[J_0(t)]  =  \mathcal{L}[1] + \sum_{n=1}^{\infty} \frac{(-1)^n}{2^{2n}(n!)^2}\mathcal{L}[t^{2n}]$ (where we’ve been careful to separate the zero-order term from the sum because we want to use TE 3, which is stated to be valid for positive integers) 

$\begin{eqnarray}
& \displaystyle \underset{\text{TE 1 & 3}}{=} & \frac1s + \sum_{n=1}^{\infty} \frac{(-1)^n(2n)!}{2^{2n}(n!)^2s^{2n+1}} \\
& = & \frac1s\left[1 + \sum_{n=1}^{\infty} \frac{(-1)^n\prod_{k=1}^n(2k)(2k-1)}{2^{2n}(n!)^2 s^{2n}}\right] \\
& = & \frac1s\left[1 + \sum_{n=1}^{\infty} \frac{(-1)^n \cancel{2^{2n}}\cancel{n!}\prod_{k=1}^n(k-\frac12)}{\cancel{2^{2n}}\cancel{n!}n! s^{2n}}\right] \\
& = & \frac1s \sum_{n=0}^{\infty} \frac{(-1)^n \prod_{k=1}^n(k-\frac12)}{n! s^{2n}} \\
& = & \frac1s \sum_{n=0}^{\infty} \binom{n-\frac12}{n}(-s^{-2})^n  \\
& = & \frac1s \frac1{\sqrt{1-(-1/s^2)}} \\
& = & (s^2 + 1)^{-1/2} ~~~~~~~~~~ \blacksquare
\end{eqnarray}$
<br><br>

For Problems 30 & 33, use the result of 28b)&mdash;$\mathcal{L}[(-t)^nf(t)] = F^{(n)}(s)$, where $F(s) = \mathcal{L}[f(t)]$&mdash;to calculate the Laplace transforms of the given functions.

<a name="P30" class="goback" onclick="winhisback()">__30__)</a>
$t^2\sin bt$

<b>Sln</b>: $t^2\sin bt = (-t)^2f(t)$ where $f(t) = \sin bt \therefore$

 $\mathcal{L}[t^2\sin bt] = (\mathcal{L}[\sin bt])’’ = \displaystyle \left(\frac{b}{s^2+b^2}\right)’’ = b\left[-2s(s^2+b^2)^{-2}\right]’ = -2b\left[(s^2+b^2)^{-2} - 4s^2(s^2+b^2)^{-3}\right] =$ $$\boxed{\frac{2b(3s^2-b^2)}{(s^2+b^2)^3}}$$
<br><br>

<a name="P33" class="goback" onclick="winhisback()">__33__)</a>
$te^{at}\sin bt$

<b>Sln</b>: $te^{at}\sin bt = -(-t)^1f(t)$ where $f(t) = e^{at}\sin bt \therefore$

$\mathcal{L}[te^{at}\sin bt] = -(\mathcal{L}[e^{at}\sin bt])’ = \displaystyle -\left(\frac{b}{(s-a)^2 + b^2}\right)’ = -2(-b)((s-a)^2 + b^2)^{-2}(s-a) = \boxed{\frac{2b(s-a)}{\left[(s-a)^2+b^2\right]^2}}$ 
<br><br>

<a name="P36" class="goback" onclick="winhisback()">__36__)</a>
Use the result of Problem 28b) to find the differential equation satisfied by the Laplace transform, $Y(s)$, of the solution, $y(t)$, of the following IVP’s:

<b>a)</b> $y’’ - ty = 0;~~y(0) = 1,~y’(0) = 0$

<b>Sln</b>: $\mathcal{L}[0] = 0 = \mathcal{L}[y’’ - ty] = s^2Y - sy(0) - y’(0) + Y’ = Y’ + s^2Y - s \implies \boxed{Y’ +s ^2Y = s}$
<br><br>

<b>b)</b> $(1-t^2)y’’ - 2ty’ + \alpha(\alpha+1)y = 0;~~y(0)=0,~y’(0)=1$

<b>Sln</b>: $\mathcal{L}[0] = 0 = \mathcal{L}[y’’-t^2y’’ - 2ty’ + \alpha(\alpha+1)y] = s^2Y - sy(0) - y’(0) - (\mathcal{L}[y’’])’’ + 2(\mathcal{L}[y’])’ + \alpha(\alpha+1)Y$

$~= s^2Y - 1 - (s^2Y - 1)’’ + 2(sY)’ + \alpha(\alpha+1)Y = s^2Y - 1 - (s^2Y’ + 2sY)’ + 2(sY’+Y) + \alpha(\alpha+1)Y \\~= s^2Y - 1 - (s^2Y’’ + 2sY’ + \cancel{2sY’} + \cancel{2Y}) + \cancel{2sY’}+ \cancel{2Y} + \alpha(\alpha+1)Y \implies \\
\boxed{s^2Y’’ + 2sY’ - [s^2+\alpha(\alpha+1)]Y = -1}$
<br><br>

### Please Donate:
<table>
  <tr style="border: none; background: transparent;">
    <td style="border: none;">
      <b>Venmo: @David-Goldsmith-13</b>
    </td>
    <td style="border: none;">
      <form action="https://www.paypal.com/cgi-bin/webscr"
            method="post"><input name="cmd"
            value="_xclick" type="hidden"> <input name="business"
            value="dgoldsmith_89@alumni.brown.edu" type="hidden"> <input
            name="item_name" value="SelectedSolutions Donation"
            type="hidden"> <input name="cn" value="Special Instructions
            (optional" type="hidden"> <input
            src="https://www.paypal.com/images/x-click-but04.gif"
            name="submit" alt="Make payments with PayPal - it's fast,
            free and secure!" align="middle" border="0" type="image"></form>
    </td>
  </tr>
</table>
